snap

io/IIO2.fst
@@ -22,8 +22,9 @@ let dm_iio' = dm_iio unit trivial_hist
 
 type gio (flag:bool) = t:dm_iio'{contains t ==> flag} // if the tree contains GetTrace, then the flag must be true
 type gio_arr (flag1:bool) (flag2:bool{flag1 ==> flag2}) = 
-  cin:dm_iio' -> 
-    cout:dm_iio'{(contains cin ==> contains cout) /\ ((contains cin ==> flag1) ==> (contains cout ==> flag2))}
+  #flag3:bool{flag1 ==> flag3} -> 
+    gio flag3 -> gio (flag2 || flag3) // l2 U (l3 \ l1)
+    //&& dm_iio'{(contains cin ==> contains cout) /\ ((contains cin ==> flag1) ==> (contains cout ==> flag2))}
 
 let gio_arr_apply (#flag1:bool) (#flag2:bool{flag1 ==> flag2}) (f:gio_arr flag1 flag2) (x:gio 'flag3) : Pure (gio (flag2 || 'flag3))
   (requires (flag1 ==> 'flag3)) 
@@ -45,10 +46,34 @@ assume val f3 : gio_arr true true
 assume val c1 : gio true
 assume val c2 : gio false
 
+[@@expect_failure]
+let test1' : gio false = gio_arr_apply f1 c1
 let test1 : gio true = gio_arr_apply f1 c1
+[@@expect_failure]
+let test2' : gio false = gio_arr_apply f2 c1
 let test2 : gio true = gio_arr_apply f2 c1
+[@@expect_failure]
+let test3' : gio false = gio_arr_apply f3 c1
 let test3 : gio true = gio_arr_apply f3 c1
-let test4 : gio true = gio_arr_apply f1 c2
+let test4' : gio true = gio_arr_apply f1 c2
+let test4 : gio false = gio_arr_apply f1 c2
+[@@expect_failure]
+let test5' : gio false = gio_arr_apply f2 c2
 let test5 : gio true = gio_arr_apply f2 c2
 [@@expect_failure]
 let test6 : gio true = gio_arr_apply f3 c2
+
+(** *** Lift from IO to GIO *)
+let dm_io' = dm_io unit trivial_hist
+
+type prog_s = gio false -> gio false
+type prog_i = gio_arr false false
+
+val comp0 : prog_s -> prog_i
+let comp0 p #f c = p c
+
+type prog_t = gio_arr true true 
+
+val comp1 : prog_i -> prog_t
+let comp1 p (c:gio true) =
+  gio_arr_apply p c
